WIP - trying to add bmatch on Sound.skenv

proof/UnreachC.v
@@ -562,9 +562,25 @@ Definition definitive_initializer (init: list init_data) : bool :=
   | _ => true
   end.
 
+Require Import ValueAnalysis ValueDomain.
+
 Inductive skenv (su: Unreach.t) (m0: mem) (ske: SkEnv.t): Prop :=
 | skenv_intro
     (PUB: su.(ge_nb) = ske.(Genv.genv_next))
+    (BMATCH: forall
+        id blk gv
+        (SYMB: ske.(Genv.find_symbol) id = Some blk)
+        (GVAR: ske.(Genv.find_var_info) blk = Some gv)
+        (GRO: gv.(gvar_readonly))
+        (GVOL: ~ gv.(gvar_volatile))
+        (GDEF: definitive_initializer gv.(gvar_init))
+
+        ske_proj keep
+        (PROJ: SkEnv.project_spec ske keep ske_proj)
+        bc
+        (GMATCH: genv_match bc ske_proj)
+      ,
+        <<BMATCH: bmatch bc m0 blk (store_init_data_list (ablock_init Pbot) 0 gv.(gvar_init))>>)
     (RO: forall
         blk gv
         (GVAR: ske.(Genv.find_var_info) blk = Some gv)
@@ -710,15 +726,22 @@ Next Obligation.
     + ii; ss.
     + ss. u in *. erewrite <- Genv.init_mem_genv_next; eauto. folder. refl.
   - econs; eauto; ss.
-  - econs; eauto; cycle 1.
+  - econs; eauto; cycle 2.
     { subst skenv. u in *. erewrite Genv.init_mem_genv_next; eauto. refl. }
-    ii. u in *. subst skenv.
-    hexploit Genv.init_mem_characterization; eauto. intro CHAR. des.
-    hexploit Genv.init_mem_characterization_gen; eauto. intro X. r in X.
-    unfold Genv.find_var_info in *. des_ifs.
-    exploit (X blk (Gvar gv)); eauto. intro GEN; des.
-    unfold Genv.perm_globvar in *. des_ifs.
-    esplits; eauto.
+    + u in MEM. u in skenv.
+
+      ii. unfold Genv.init_mem in *. subst skenv.
+      exploit alloc_globals_match; eauto.
+      { ss. }
+      { ii. uge. des_ifs. ss. rewrite PTree.gempty in *. clarify. }
+      { destruct (gvar_volatile gv) eqn:T; ss. }
+    + ii. u in *. subst skenv.
+      hexploit Genv.init_mem_characterization; eauto. intro CHAR. des.
+      hexploit Genv.init_mem_characterization_gen; eauto. intro X. r in X.
+      unfold Genv.find_var_info in *. des_ifs.
+      exploit (X blk (Gvar gv)); eauto. intro GEN; des.
+      unfold Genv.perm_globvar in *. des_ifs.
+      esplits; eauto.
 Qed.
 Next Obligation.
   inv LE.
@@ -727,48 +750,118 @@ Next Obligation.
 Qed.
 Next Obligation.
   inv MLE.
-  inv SKE. econs; eauto; cycle 1.
+  inv SKE. econs; eauto; cycle 2.
   { etrans; eauto. eauto with mem. }
-  ii. exploit RO0; eauto. i; des.
-  esplits; eauto.
-  - ii. eapply PERM0; eauto. eapply PERM; eauto.
-    { r. eapply Plt_Ple_trans; eauto.
-      admit "ez - GVAR/genv_defs_range".
-    }
-  - eapply Genv.load_store_init_data_invariant; try apply LABLE; eauto.
-    unfold Genv.find_var_info in *. des_ifs.
-    i. eapply Mem.load_unchanged_on_1; try apply RO; eauto.
-    { admit "ez - Heq/genv_defs_range/NB". }
-    ii. exploit PERM0; eauto. i; des. inv ORD.
+  - ii. r.
+    eapply bmatch_inv.
+    { eapply BMATCH; et. }
+    i. eapply Mem.loadbytes_unchanged_on_1; try apply RO; eauto.
+    { clear - SYMB NB. admit "ez". }
+    ii. exploit RO0; eauto. i; des. exploit PERM0; eauto. i; des.
+    inv ORD.
+  - ii. exploit RO0; eauto. i; des.
+    esplits; eauto.
+    + ii. eapply PERM0; eauto. eapply PERM; eauto.
+      { r. eapply Plt_Ple_trans; eauto.
+        admit "ez - GVAR/genv_defs_range".
+      }
+    + eapply Genv.load_store_init_data_invariant; try apply LABLE; eauto.
+      unfold Genv.find_var_info in *. des_ifs.
+      i. eapply Mem.load_unchanged_on_1; try apply RO; eauto.
+      { admit "ez - Heq/genv_defs_range/NB". }
+      ii. exploit PERM0; eauto. i; des. inv ORD.
 Qed.
 Next Obligation.
   exploit SkEnv.project_spec_preserves_wf; eauto. intro WFSMALL.
   inv SKE. inv LE. inv WFSMALL.
-  econs; eauto; swap 2 3.
+  econs; eauto; swap 2 4.
   { congruence. }
   { etrans; eauto. rewrite NEXT. refl. }
-  ii.
-  unfold Genv.find_var_info in *. des_ifs.
-  exploit DEFSYMB; eauto. i; des.
-  destruct (classic (defs0 id)); cycle 1.
-  { exploit SYMBDROP; eauto. i; des. clarify. }
-  exploit SYMBKEEP; eauto. i; des. rewrite H in *. symmetry in H1.
-  inv WF.
-  exploit SYMBDEF0; eauto. intro DEF; des.
-  exploit DEFKEEP; eauto.
-  { eapply Genv.find_invert_symbol; eauto. }
-  intro DEF2; des. rewrite DEF in *. clarify.
-  exploit RO; eauto.
-  { rewrite DEF. ss. }
-  i; des.
-  esplits; eauto.
+  - ii.
+    unfold Genv.find_var_info in *. des_ifs.
+    exploit DEFSYMB; eauto. i; des.
+    destruct (classic (defs0 id)); cycle 1.
+    { exploit SYMBDROP; eauto. i; des. clarify. }
+    exploit SYMBKEEP; eauto. i; des. rewrite H in *. symmetry in H1.
+    inv WF.
+    exploit SYMBDEF0; eauto. intro DEF; des.
+    exploit DEFKEEP; eauto.
+    { eapply Genv.find_invert_symbol; eauto. }
+    intro DEF2; des. rewrite DEF in *. clarify.
+    exploit RO; eauto.
+    { rewrite DEF. ss. }
+    i; des.
+    esplits; eauto.
 
-  clear - LABLE SYMBKEEP.
-  destruct gv; ss. clear_tac. revert LABLE. generalize (0%Z) as ofs. i.
-  ginduction gvar_init; ii; ss.
-  des_ifs; des; esplits; eauto.
-  rewrite SYMBKEEP; eauto.
-  admit "hard - we need good_prog".
+    clear - LABLE SYMBKEEP.
+    destruct gv; ss. clear_tac. revert LABLE. generalize (0%Z) as ofs. i.
+    ginduction gvar_init; ii; ss.
+    des_ifs; des; esplits; eauto.
+    rewrite SYMBKEEP; eauto.
+    admit "hard - we need good_prog".
+  - (** copied from above **)
+    ii.
+    unfold Genv.find_var_info in *. des_ifs.
+    (* exploit DEFSYMB; eauto. i; des. *)
+    destruct (classic (defs0 id)); cycle 1.
+    { exploit SYMBDROP; eauto. i; des. clarify. }
+    exploit SYMBKEEP; eauto. i; des. rewrite SYMB in *. symmetry in H0.
+    inv WF.
+    exploit SYMBDEF0; eauto. intro DEF; des.
+    exploit DEFKEEP; eauto.
+    { eapply Genv.find_invert_symbol; eauto. }
+    intro DEF2; des. rewrite DEF in *. clarify.
+
+    assert(BCLINK: exists bc_link, genv_match bc_link skenv_link /\
+                                   <<IMG: bc_link.(bc_img) = (fun blk =>
+                                                                match (Genv.invert_symbol skenv_link blk) with
+                                                                | Some id => BCglob id
+                                                                | _ => BCother
+                                                                end)>>).
+    { unshelve eexists (BC (fun blk => match (Genv.invert_symbol skenv_link blk) with
+                                       | Some id => BCglob id
+                                       | _ => BCother
+                                       end) _ _); cycle 2.
+      { unfold genv_match. s. split; cycle 1.
+        { refl. }
+        split.
+        - split; intro T.
+          + apply Genv.find_invert_symbol in T. des_ifs.
+          + des_ifs. apply Genv.invert_find_symbol in Heq. des_ifs.
+        - i.
+          split; des_ifs.
+      }
+      { ss. ii. des_ifs. }
+      { ss. ii. des_ifs. apply_all_once Genv.invert_find_symbol. congruence. }
+    }
+    des.
+    eapply bmatch_incr with (bc2 := bc_link).
+    eapply BMATCH; try apply BCLINK; eauto.
+    { rewrite IMG. apply Genv.find_invert_symbol in H0. des_ifs. }
+    { rewrite DEF. ss. }
+    { rr. rr in GMATCH. des. esplits; ss; eauto.
+      - i. etrans; cycle 1.
+        { eapply GMATCH. }
+        
+    }
+
+    exploit RO; eauto.
+    { rewrite DEF. ss. }
+    i; des.
+    esplits; eauto.
+
+    exploit BMATCH; eauto.
+    { rewrite DEF. ss. }
+    i; des.
+    esplits; eauto.
+    clear - LABLE SYMBKEEP.
+    destruct gv; ss. clear_tac. revert LABLE. generalize (0%Z) as ofs. i.
+    ginduction gvar_init; ii; ss.
+    des_ifs; des; esplits; eauto.
+    rewrite SYMBKEEP; eauto.
+    admit "hard - we need good_prog".
+  - ii. eapply BMATCH; eauto.
+    +
 Qed.
 Next Obligation.
   split; i; inv H; ss.
